fstar/treedem/MLS.TreeDEM.Message.Framing.fst
@@ -21,44 +21,44 @@ let compute_message_confirmation_tag #bytes #cb confirmation_key confirmed_trans
 val knows_group_context: #bytes:Type0 -> {|bytes_like bytes|} -> sender_nt bytes -> bool
 let knows_group_context #bytes #bl sender = NT.S_member? sender || NT.S_new_member_commit? sender
 
-val compute_tbs: #bytes:Type0 -> {|bytes_like bytes|} -> wire_format_nt -> content:mls_content_nt bytes -> group_context:option (group_context_nt bytes){Some? group_context <==> knows_group_context content.sender} -> mls_content_tbs_nt bytes
+val compute_tbs: #bytes:Type0 -> {|bytes_like bytes|} -> wire_format_nt -> content:framed_content_nt bytes -> group_context:option (group_context_nt bytes){Some? group_context <==> knows_group_context content.sender} -> framed_content_tbs_nt bytes
 let compute_tbs #bytes #bl wire_format content group_context =
   ({
     wire_format;
     content;
     group_context = (match group_context with | Some gc -> gc | None -> ());
-  } <: mls_content_tbs_nt bytes)
+  } <: framed_content_tbs_nt bytes)
 
-val compute_tbm: #bytes:Type0 -> {|bytes_like bytes|} -> content:mls_content_nt bytes -> mls_content_auth_data_nt bytes content.content.content_type -> group_context:option (group_context_nt bytes){Some? group_context <==> knows_group_context content.sender} -> mls_content_tbm_nt bytes
+val compute_tbm: #bytes:Type0 -> {|bytes_like bytes|} -> content:framed_content_nt bytes -> framed_content_auth_data_nt bytes content.content.content_type -> group_context:option (group_context_nt bytes){Some? group_context <==> knows_group_context content.sender} -> authenticated_content_tbm_nt bytes
 let compute_tbm #bytes #bl content auth group_context =
-  let content_tbs = compute_tbs WF_mls_plaintext content group_context in
+  let content_tbs = compute_tbs WF_mls_public_message content group_context in
   ({
     content_tbs;
     auth;
-  } <: mls_content_tbm_nt bytes)
+  } <: authenticated_content_tbm_nt bytes)
 
-val compute_message_signature: #bytes:Type0 -> {|crypto_bytes bytes|} -> sign_private_key bytes -> sign_nonce bytes -> wire_format_nt -> content:mls_content_nt bytes -> group_context:option (group_context_nt bytes){Some? group_context <==> knows_group_context content.sender} -> result (sign_signature bytes)
+val compute_message_signature: #bytes:Type0 -> {|crypto_bytes bytes|} -> sign_private_key bytes -> sign_nonce bytes -> wire_format_nt -> content:framed_content_nt bytes -> group_context:option (group_context_nt bytes){Some? group_context <==> knows_group_context content.sender} -> result (sign_signature bytes)
 let compute_message_signature #bytes #cb sk rand wire_format msg group_context =
   let tbs = compute_tbs wire_format msg group_context in
-  let serialized_tbs: bytes = serialize (mls_content_tbs_nt bytes) tbs in
-  if not (length serialized_tbs < pow2 30 && sign_with_label_pre #bytes "MLSContentTBS" (length #bytes serialized_tbs)) then error "compute_message_signature: tbs too long"
+  let serialized_tbs: bytes = serialize (framed_content_tbs_nt bytes) tbs in
+  if not (length serialized_tbs < pow2 30 && sign_with_label_pre #bytes "FramedContentTBS" (length #bytes serialized_tbs)) then error "compute_message_signature: tbs too long"
   else (
-    return (sign_with_label sk "MLSContentTBS" serialized_tbs rand)
+    return (sign_with_label sk "FramedContentTBS" serialized_tbs rand)
   )
 
-val check_message_signature: #bytes:Type0 -> {|crypto_bytes bytes|} -> sign_public_key bytes -> sign_signature bytes -> wire_format_nt -> content:mls_content_nt bytes -> group_context:option (group_context_nt bytes){Some? group_context <==> knows_group_context content.sender} -> result bool
+val check_message_signature: #bytes:Type0 -> {|crypto_bytes bytes|} -> sign_public_key bytes -> sign_signature bytes -> wire_format_nt -> content:framed_content_nt bytes -> group_context:option (group_context_nt bytes){Some? group_context <==> knows_group_context content.sender} -> result bool
 let check_message_signature #bytes #cb pk signature wire_format msg group_context =
   let tbs = compute_tbs wire_format msg group_context in
-  let serialized_tbs: bytes = serialize (mls_content_tbs_nt bytes) tbs in
-  if not (length serialized_tbs < pow2 30 && sign_with_label_pre #bytes "MLSContentTBS" (length #bytes serialized_tbs)) then error "check_message_signature: tbs too long"
+  let serialized_tbs: bytes = serialize (framed_content_tbs_nt bytes) tbs in
+  if not (length serialized_tbs < pow2 30 && sign_with_label_pre #bytes "FramedContentTBS" (length #bytes serialized_tbs)) then error "check_message_signature: tbs too long"
   else (
-    return (verify_with_label pk "MLSContentTBS" serialized_tbs signature)
+    return (verify_with_label pk "FramedContentTBS" serialized_tbs signature)
   )
 
-val compute_message_membership_tag: #bytes:Type0 -> {|crypto_bytes bytes|} -> bytes -> content:mls_content_nt bytes -> mls_content_auth_data_nt bytes content.content.content_type -> group_context:option (group_context_nt bytes){Some? group_context <==> knows_group_context content.sender} -> result (lbytes bytes (hmac_length #bytes))
+val compute_message_membership_tag: #bytes:Type0 -> {|crypto_bytes bytes|} -> bytes -> content:framed_content_nt bytes -> framed_content_auth_data_nt bytes content.content.content_type -> group_context:option (group_context_nt bytes){Some? group_context <==> knows_group_context content.sender} -> result (lbytes bytes (hmac_length #bytes))
 let compute_message_membership_tag #bytes #cb membership_key msg auth group_context =
   let tbm = compute_tbm msg auth group_context in
-  let serialized_tbm = serialize (mls_content_tbm_nt bytes) tbm in
+  let serialized_tbm = serialize (authenticated_content_tbm_nt bytes) tbm in
   hmac_hmac membership_key serialized_tbm
 
 //TODO: this function should be refactored
@@ -87,15 +87,15 @@ let message_compute_auth #bytes #cb msg sk rand group_context confirmation_key i
 (*** From/to plaintext ***)
 
 //TODO check membership tag
-val message_plaintext_to_message: #bytes:Type0 -> {|bytes_like bytes|} -> mls_plaintext_nt bytes -> mls_authenticated_content_nt bytes
+val message_plaintext_to_message: #bytes:Type0 -> {|bytes_like bytes|} -> public_message_nt bytes -> authenticated_content_nt bytes
 let message_plaintext_to_message #bytes #bl pt =
   {
-    wire_format = WF_mls_plaintext;
+    wire_format = WF_mls_public_message;
     content = pt.content;
     auth = pt.auth;
   }
 
-val message_to_message_plaintext: #bytes:Type0 -> {|crypto_bytes bytes|} -> membership_key:bytes -> auth_msg:mls_authenticated_content_nt bytes{auth_msg.wire_format == WF_mls_plaintext} -> group_context:option (group_context_nt bytes){Some? group_context <==> knows_group_context auth_msg.content.sender} -> result (mls_plaintext_nt bytes)
+val message_to_message_plaintext: #bytes:Type0 -> {|crypto_bytes bytes|} -> membership_key:bytes -> auth_msg:authenticated_content_nt bytes{auth_msg.wire_format == WF_mls_public_message} -> group_context:option (group_context_nt bytes){Some? group_context <==> knows_group_context auth_msg.content.sender} -> result (public_message_nt bytes)
 let message_to_message_plaintext #bytes #cb membership_key auth_msg group_context =
   let? membership_tag = (
     match auth_msg.content.sender with
@@ -109,7 +109,7 @@ let message_to_message_plaintext #bytes #cb membership_key auth_msg group_contex
     content = auth_msg.content;
     auth = auth_msg.auth;
     membership_tag;
-  } <: mls_plaintext_nt bytes)
+  } <: public_message_nt bytes)
 
 (*** From/to ciphertext ***)
 
@@ -122,64 +122,64 @@ let get_ciphertext_sample #bytes #cb ct =
     fst (unsafe_split ct len)
 
 //Used in decryption
-val message_ciphertext_to_sender_data_aad: #bytes:Type0 -> {|bytes_like bytes|} -> mls_ciphertext_nt bytes -> mls_sender_data_aad_nt bytes
+val message_ciphertext_to_sender_data_aad: #bytes:Type0 -> {|bytes_like bytes|} -> private_message_nt bytes -> sender_data_aad_nt bytes
 let message_ciphertext_to_sender_data_aad #bytes #bl ct =
   ({
     group_id = ct.group_id;
     epoch = ct.epoch;
     content_type = ct.content_type;
-  } <: mls_sender_data_aad_nt bytes)
+  } <: sender_data_aad_nt bytes)
 
 //Used in encryption
-val message_to_sender_data_aad: #bytes:Type0 -> {|bytes_like bytes|} -> mls_content_nt bytes -> mls_sender_data_aad_nt bytes
+val message_to_sender_data_aad: #bytes:Type0 -> {|bytes_like bytes|} -> framed_content_nt bytes -> sender_data_aad_nt bytes
 let message_to_sender_data_aad #bytes #bl content =
   ({
     group_id = content.group_id;
     epoch = content.epoch;
     content_type = content.content.content_type;
-  } <: mls_sender_data_aad_nt bytes)
+  } <: sender_data_aad_nt bytes)
 
-val decrypt_sender_data: #bytes:Type0 -> {|crypto_bytes bytes|} -> mls_sender_data_aad_nt bytes -> ciphertext_sample:bytes -> sender_data_secret:bytes -> encrypted_sender_data:bytes -> result (mls_sender_data_nt bytes)
+val decrypt_sender_data: #bytes:Type0 -> {|crypto_bytes bytes|} -> sender_data_aad_nt bytes -> ciphertext_sample:bytes -> sender_data_secret:bytes -> encrypted_sender_data:bytes -> result (sender_data_nt bytes)
 let decrypt_sender_data #bytes #cb ad ciphertext_sample sender_data_secret encrypted_sender_data =
   let? sender_data_key = expand_with_label sender_data_secret (string_to_bytes #bytes "key") ciphertext_sample (aead_key_length #bytes) in
   let? sender_data_nonce = expand_with_label sender_data_secret (string_to_bytes #bytes "nonce") ciphertext_sample (aead_nonce_length #bytes) in
-  let? sender_data = aead_decrypt sender_data_key sender_data_nonce (serialize (mls_sender_data_aad_nt bytes) ad) encrypted_sender_data in
-  from_option "decrypt_sender_data: malformed sender data" (parse (mls_sender_data_nt bytes) sender_data)
+  let? sender_data = aead_decrypt sender_data_key sender_data_nonce (serialize (sender_data_aad_nt bytes) ad) encrypted_sender_data in
+  from_option "decrypt_sender_data: malformed sender data" (parse (sender_data_nt bytes) sender_data)
 
-val encrypt_sender_data: #bytes:Type0 -> {|crypto_bytes bytes|} -> mls_sender_data_aad_nt bytes -> ciphertext_sample:bytes -> sender_data_secret:bytes -> mls_sender_data_nt bytes -> result bytes
+val encrypt_sender_data: #bytes:Type0 -> {|crypto_bytes bytes|} -> sender_data_aad_nt bytes -> ciphertext_sample:bytes -> sender_data_secret:bytes -> sender_data_nt bytes -> result bytes
 let encrypt_sender_data #bytes #cb ad ciphertext_sample sender_data_secret sender_data =
   let? sender_data_key = expand_with_label sender_data_secret (string_to_bytes #bytes "key") ciphertext_sample (aead_key_length #bytes) in
   let? sender_data_nonce = expand_with_label sender_data_secret (string_to_bytes #bytes "nonce") ciphertext_sample (aead_nonce_length #bytes) in
-  aead_encrypt sender_data_key sender_data_nonce (serialize (mls_sender_data_aad_nt bytes) ad) (serialize (mls_sender_data_nt bytes) sender_data)
+  aead_encrypt sender_data_key sender_data_nonce (serialize (sender_data_aad_nt bytes) ad) (serialize (sender_data_nt bytes) sender_data)
 
 // Used in decryption
-val message_ciphertext_to_ciphertext_content_aad: #bytes:Type0 -> {|bytes_like bytes|} -> ct:mls_ciphertext_nt bytes -> res:mls_ciphertext_content_aad_nt bytes{res.content_type == ct.content_type}
+val message_ciphertext_to_ciphertext_content_aad: #bytes:Type0 -> {|bytes_like bytes|} -> ct:private_message_nt bytes -> res:private_content_aad_nt bytes{res.content_type == ct.content_type}
 let message_ciphertext_to_ciphertext_content_aad #bytes #bl ct =
   ({
     group_id = ct.group_id;
     epoch = ct.epoch;
     content_type = ct.content_type;
     authenticated_data = ct.authenticated_data;
-  } <: mls_ciphertext_content_aad_nt bytes)
+  } <: private_content_aad_nt bytes)
 
-val decrypt_ciphertext_content: #bytes:Type0 -> {|crypto_bytes bytes|} -> ad:mls_ciphertext_content_aad_nt bytes -> aead_key bytes -> aead_nonce bytes -> ct:bytes -> result (mls_ciphertext_content_nt bytes ad.content_type)
+val decrypt_ciphertext_content: #bytes:Type0 -> {|crypto_bytes bytes|} -> ad:private_content_aad_nt bytes -> aead_key bytes -> aead_nonce bytes -> ct:bytes -> result (private_content_tbe_nt bytes ad.content_type)
 let decrypt_ciphertext_content #bytes #cb ad key nonce ct =
-  let? ciphertext_content = aead_decrypt key nonce (serialize (mls_ciphertext_content_aad_nt bytes) ad) ct in
-  from_option "decrypt_ciphertext_content: malformed ciphertext content" (parse (mls_ciphertext_content_nt bytes ad.content_type) ciphertext_content)
+  let? ciphertext_content = aead_decrypt key nonce (serialize (private_content_aad_nt bytes) ad) ct in
+  from_option "decrypt_ciphertext_content: malformed ciphertext content" (parse (private_content_tbe_nt bytes ad.content_type) ciphertext_content)
 
 // Used in encryption
-val message_to_ciphertext_content_aad: #bytes:Type0 -> {|bytes_like bytes|} -> content:mls_content_nt bytes -> res:mls_ciphertext_content_aad_nt bytes{res.content_type == content.content.content_type}
+val message_to_ciphertext_content_aad: #bytes:Type0 -> {|bytes_like bytes|} -> content:framed_content_nt bytes -> res:private_content_aad_nt bytes{res.content_type == content.content.content_type}
 let message_to_ciphertext_content_aad #bytes #bl content =
   ({
     group_id = content.group_id;
     epoch = content.epoch;
     content_type = content.content.content_type;
     authenticated_data = content.authenticated_data;
-  } <: mls_ciphertext_content_aad_nt bytes)
+  } <: private_content_aad_nt bytes)
 
-val encrypt_ciphertext_content: #bytes:Type0 -> {|crypto_bytes bytes|} -> ad:mls_ciphertext_content_aad_nt bytes -> aead_key bytes -> aead_nonce bytes -> (mls_ciphertext_content_nt bytes ad.content_type) -> result bytes
+val encrypt_ciphertext_content: #bytes:Type0 -> {|crypto_bytes bytes|} -> ad:private_content_aad_nt bytes -> aead_key bytes -> aead_nonce bytes -> (private_content_tbe_nt bytes ad.content_type) -> result bytes
 let encrypt_ciphertext_content #bytes #cb ad key nonce pt =
-  aead_encrypt key nonce (serialize (mls_ciphertext_content_aad_nt bytes) ad) (serialize (mls_ciphertext_content_nt bytes ad.content_type) pt)
+  aead_encrypt key nonce (serialize (private_content_aad_nt bytes) ad) (serialize (private_content_tbe_nt bytes ad.content_type) pt)
 
 val apply_reuse_guard: #bytes:Type0 -> {|crypto_bytes bytes|} -> lbytes bytes 4 -> aead_nonce bytes -> aead_nonce bytes
 let apply_reuse_guard #bytes #cb reuse_guard nonce =
@@ -189,7 +189,7 @@ let apply_reuse_guard #bytes #cb reuse_guard nonce =
   let new_nonce_head = xor nonce_head reuse_guard in
   concat #bytes new_nonce_head nonce_tail
 
-val message_ciphertext_to_message: #bytes:Type0 -> {|crypto_bytes bytes|} -> l:nat -> encryption_secret:bytes -> sender_data_secret:bytes -> mls_ciphertext_nt bytes -> result (mls_authenticated_content_nt bytes)
+val message_ciphertext_to_message: #bytes:Type0 -> {|crypto_bytes bytes|} -> l:nat -> encryption_secret:bytes -> sender_data_secret:bytes -> private_message_nt bytes -> result (authenticated_content_nt bytes)
 let message_ciphertext_to_message #bytes #cb l encryption_secret sender_data_secret ct =
   let? sender_data = (
     let sender_data_ad = message_ciphertext_to_sender_data_aad ct in
@@ -218,7 +218,7 @@ let message_ciphertext_to_message #bytes #cb l encryption_secret sender_data_sec
     decrypt_ciphertext_content ciphertext_content_ad key patched_nonce ct.ciphertext
   ) in
   return ({
-    wire_format = WF_mls_ciphertext;
+    wire_format = WF_mls_private_message;
     content = {
       group_id = ct.group_id;
       epoch = ct.epoch;
@@ -233,7 +233,7 @@ let message_ciphertext_to_message #bytes #cb l encryption_secret sender_data_sec
       signature = ciphertext_content.data.auth.signature;
       confirmation_tag = ciphertext_content.data.auth.confirmation_tag;
     };
-  } <: mls_authenticated_content_nt bytes)
+  } <: authenticated_content_nt bytes)
 
 val get_serializeable_bytes: #bytes:Type0 -> {|bytes_like bytes|} -> bytes -> result (mls_bytes bytes)
 let get_serializeable_bytes #bytes #bl b =
@@ -243,13 +243,13 @@ let get_serializeable_bytes #bytes #bl b =
     return b
   )
 
-val message_to_message_ciphertext: #bytes:Type0 -> {|crypto_bytes bytes|} -> ratchet_state bytes -> lbytes bytes 4 -> bytes -> msg:mls_authenticated_content_nt bytes{msg.wire_format == WF_mls_ciphertext} -> result (mls_ciphertext_nt bytes & ratchet_state bytes)
+val message_to_message_ciphertext: #bytes:Type0 -> {|crypto_bytes bytes|} -> ratchet_state bytes -> lbytes bytes 4 -> bytes -> msg:authenticated_content_nt bytes{msg.wire_format == WF_mls_private_message} -> result (private_message_nt bytes & ratchet_state bytes)
 let message_to_message_ciphertext #bytes #cb ratchet reuse_guard sender_data_secret auth_msg =
   let? ciphertext = (
     let? key_nonce = ratchet_get_key ratchet in
     let key = key_nonce.key in
     let patched_nonce = apply_reuse_guard reuse_guard key_nonce.nonce in
-    let ciphertext_content: mls_ciphertext_content_nt bytes (auth_msg.content.content.content_type) = {
+    let ciphertext_content: private_content_tbe_nt bytes (auth_msg.content.content.content_type) = {
       data = {
         content = auth_msg.content.content.content;
         auth = auth_msg.auth;
@@ -284,4 +284,4 @@ let message_to_message_ciphertext #bytes #cb ratchet reuse_guard sender_data_sec
     authenticated_data = auth_msg.content.authenticated_data;
     encrypted_sender_data = encrypted_sender_data;
     ciphertext = ciphertext;
-  } <: mls_ciphertext_nt bytes), new_ratchet)
+  } <: private_message_nt bytes), new_ratchet)
